Clean up Coq code.

PosTree.v
@@ -1,5 +1,12 @@
 Require Export InfixGrammar.
-Require Import Utils.
+
+(* 
+  In this section we define a pos_tree. Such a tree, which we can also call an indexed
+  parse tree, or positional parse tree, is an extension to an ordinary parse_tree. Each
+  lexical symbol and operand symbol gets assigned a natural number, representing the index
+  of the symbol. The goal is that each index will also be the index of the symbol that ends
+  up in the yield of the tree.
+*)
 
 Section PosTree.
 Context {L O : Type}.
@@ -10,6 +17,8 @@ Inductive pos_tree :=
 
 Implicit Types pt : pos_tree.
 
+(* Definition of what it means for a pos_tree to be well-formed between a number n0 and n.
+   n0 is the start index (inclusive) and n is the final index (exclusive). *)
 Inductive wf_pos_tree : nat -> pos_tree -> nat -> Prop :=
   | Wfpos_PANode i l :
       wf_pos_tree i (PANode l i) (S i)
@@ -18,24 +27,16 @@ Inductive wf_pos_tree : nat -> pos_tree -> nat -> Prop :=
       wf_pos_tree (S j) pt2 k ->
       wf_pos_tree i (PINode pt1 o j pt2) k.
 
-Inductive nth_symbol n : (L + O) -> pos_tree -> Prop :=
-  | L_nth l :
-      nth_symbol n (inl l) (PANode l n)
-  | O_nth o pt1 pt2 :
-      nth_symbol n (inr o) (PINode pt1 o n pt2)
-  | Symbol_nth1 s pt1 pt2 o i :
-      nth_symbol n s pt1 ->
-      nth_symbol n s (PINode pt1 o i pt2)
-  | Symbol_nth2 s pt1 pt2 o i :
-      nth_symbol n s pt2 ->
-      nth_symbol n s (PINode pt1 o i pt2).
-
+(* This function transforms a pos_tree into and ordinary parse_tree by removing all
+   indices. *)
 Fixpoint unpos pt : parse_tree :=
   match pt with
   | PANode l _ => ANode l
   | PINode pt1 o _ pt2 => INode (unpos pt1) o (unpos pt2)
   end.
-
+ 
+(* This function transforms an ordinary parse_tree into a pos_tree pt and number n, given
+   some start index n0, such that the pos_tree is well-formed between n0 and n. *)
 Fixpoint pos t (n0 : nat) : (pos_tree * nat) :=
   match t with
   | ANode l => (PANode l n0, S n0)
@@ -45,15 +46,30 @@ Fixpoint pos t (n0 : nat) : (pos_tree * nat) :=
       (PINode pt1 o i pt2, n)
   end.
 
+(* (ith_symbol i s pt) states that symbol s is in pt with index i. *)
+Inductive ith_symbol i : (L + O) -> pos_tree -> Prop :=
+  | L_ith l :
+      ith_symbol i (inl l) (PANode l i)
+  | O_ith o pt1 pt2 :
+      ith_symbol i (inr o) (PINode pt1 o i pt2)
+  | S_ith_l s pt1 pt2 o j :
+      ith_symbol i s pt1 ->
+      ith_symbol i s (PINode pt1 o j pt2)
+  | S_ith_r s pt1 pt2 o j :
+      ith_symbol i s pt2 ->
+      ith_symbol i s (PINode pt1 o j pt2).
+
+(* Two pos_trees are position equivalent if and only if they have the same symbols on the
+   same indices. *)
 Definition pos_equivalent pt1 pt2 : Prop :=
-  forall s i, nth_symbol i s pt1 <-> nth_symbol i s pt2.
+  forall s i, ith_symbol i s pt1 <-> ith_symbol i s pt2.
 
 End PosTree.
 
 Create HintDb pos_tree.
 Hint Resolve Wfpos_PANode : pos_tree.
 Hint Resolve Wfpos_PINode : pos_tree.
-Hint Resolve L_nth : pos_tree.
-Hint Resolve O_nth : pos_tree.
-Hint Resolve Symbol_nth1 : pos_tree.
-Hint Resolve Symbol_nth2 : pos_tree.
+Hint Resolve L_ith : pos_tree.
+Hint Resolve O_ith : pos_tree.
+Hint Resolve S_ith_l : pos_tree.
+Hint Resolve S_ith_r : pos_tree.
