Reordering.v
@@ -10,6 +10,7 @@ Implicit Types s : L + O.
 Implicit Types t : @parse_tree L O.
 Implicit Types pt : @pos_tree L O.
 
+(* One-step reordering for parse_trees. *)
 Inductive reorder_step : parse_tree -> parse_tree -> Prop :=
   | RI_LR t11 o1 t12 o t2 :
       reorder_step (INode (INode t11 o1 t12) o t2)
@@ -17,36 +18,17 @@ Inductive reorder_step : parse_tree -> parse_tree -> Prop :=
   | RI_RL t1 o t21 o2 t22 :
       reorder_step (INode t1 o (INode t21 o2 t22))
                    (INode (INode t1 o t21) o2 t22)
-  | RI_t1 t1 o t2 t1' :
+  | RI_t_l t1 o t2 t1' :
       reorder_step t1 t1' ->
       reorder_step (INode t1 o t2) (INode t1' o t2)
-  | RI_t2 t1 o t2 t2' :
+  | RI_t_r t1 o t2 t2' :
       reorder_step t2 t2' ->
       reorder_step (INode t1 o t2) (INode t1 o t2').
 
+(* Reflexive and transitive closure of reordering parse_trees. *)
 Definition reorder := rtc reorder_step.
 
-Ltac super_simpl := try simpl in *; try simplify_list_eq; try reflexivity.
-
-Lemma reorder_step_preserves_yields t t' :
-  reorder_step t t' -> yield t = yield t'.
-Proof.
-  intros. induction H; super_simpl.
-  - rewrite IHreorder_step. reflexivity.
-  - rewrite IHreorder_step. reflexivity.
-Qed.
-
-Lemma reorder_preserves_yield t t' :
-  reorder t t' -> yield t = yield t'.
-Proof.
-  unfold reorder. intros.
-  induction H.
-  - reflexivity.
-  - rewrite <- IHrtc.
-    apply reorder_step_preserves_yields.
-    assumption.
-Qed.
-
+(* Analogous definition of reordering, but now for pos_trees. *)
 Inductive reorder_step_pos : pos_tree -> pos_tree -> Prop :=
   | PRI_LR pt11 o1 i1 pt12 o i pt2 :
       reorder_step_pos (PINode (PINode pt11 o1 i1 pt12) o i pt2)
@@ -54,15 +36,25 @@ Inductive reorder_step_pos : pos_tree -> pos_tree -> Prop :=
   | PRI_RL pt1 o i pt21 o2 i2 pt22 :
       reorder_step_pos (PINode pt1 o i (PINode pt21 o2 i2 pt22))
                       (PINode (PINode pt1 o i pt21) o2 i2 pt22)
-  | PRI_pt1 pt1 o i pt2 pt1' :
+  | PRI_pt_l pt1 o i pt2 pt1' :
       reorder_step_pos pt1 pt1' ->
       reorder_step_pos (PINode pt1 o i pt2) (PINode pt1' o i pt2)
-  | PRI_pt2 pt1 o i pt2 pt2' :
+  | PRI_pt_r pt1 o i pt2 pt2' :
       reorder_step_pos pt2 pt2' ->
       reorder_step_pos (PINode pt1 o i pt2) (PINode pt1 o i pt2').
 
 Definition reorder_pos := rtc reorder_step_pos.
 
 End Reordering.
+
+Create HintDb reordering.
+Hint Resolve RI_LR : reordering.
+Hint Resolve RI_RL : reordering.
+Hint Resolve RI_t_l : reordering.
+Hint Resolve RI_t_r : reordering.
+Hint Resolve PRI_LR : reordering.
+Hint Resolve PRI_RL : reordering.
+Hint Resolve PRI_pt_l : reordering.
+Hint Resolve PRI_pt_r : reordering.
 
 
