PosTreeTheorems.v
@@ -9,8 +9,9 @@ Implicit Types s : L + O.
 Implicit Types t : @parse_tree L O.
 Implicit Types pt : @pos_tree L O.
 
-Lemma wf_pos_tree_size i j pt : 
-  wf_pos_tree i pt j -> j = i + length (yield (unpos pt)). 
+(* If a pos_tree is well-formed between n0 and n, then its size is n - n0. *)
+Lemma wf_pos_tree_size n0 n pt : 
+  wf_pos_tree n0 pt n -> n = n0 + length (yield (unpos pt)). 
 Proof.
   intros.
   induction H; simpl.
@@ -20,51 +21,62 @@ Proof.
     lia.
 Qed.
 
-Lemma symbol_between_indices i0 pt n i s :
-  wf_pos_tree i0 pt n -> nth_symbol i s pt -> le i0 i /\ i < n.
+(* If a symbol is in a well-formed pos_tree between n0 and n in i, then n0 <= i < n. *)
+Lemma symbol_between_indices n0 pt n i s :
+  wf_pos_tree n0 pt n -> ith_symbol i s pt -> le n0 i /\ i < n.
 Proof.
-  revert i0 i n.
-  induction pt; intros.
+  intro.
+  induction H; intros.
+  (* CASE: pt = (l, n0) *)
   - inv H.
-    inv H0.
     lia.
-  - inv H.
-    apply wf_pos_tree_size in H7 as ?.
-    apply wf_pos_tree_size in H8 as ?.
-    inv H0.
-    + split; lia.
-    + eapply IHpt1 in H7; [|eassumption].
-      destruct H7.
-      split; lia.
-    + eapply IHpt2 in H8; [|eassumption].
-      destruct H8.
-      split; lia.
+  (* CASE: pt = [pt1 (o, j) pt2] *)
+  - apply wf_pos_tree_size in H as ?.
+    apply wf_pos_tree_size in H0 as ?.
+    inv H1.
+    (* CASE: s = o *)
+    + lia.
+    (* CASE: s is in pt1 *)
+    + apply IHwf_pos_tree1 in H6.
+      lia.
+    (* CASE: s is in pt2 *)
+    + apply IHwf_pos_tree2 in H6.
+      lia.
 Qed.
 
+(* If a symbol s is in a well-formed pos_tree between n0 and n in i, then s in the
+   (i - n0)th position of the yield. *)
 Lemma pos_yield pt n0 n s i :
   wf_pos_tree n0 pt n ->
-  nth_symbol i s pt -> (yield (unpos pt)) !! (i - n0) = Some s.
+  ith_symbol i s pt -> (yield (unpos pt)) !! (i - n0) = Some s.
 Proof.
+  (* By induction over well-formedness of pt *)
   intros. induction H.
+  (* CASE: pt = (l, n0) and yield(pt) = l *)
   - inv H0.
     replace (i0 - i0) with 0; [|lia].
     reflexivity.
+  (* CASE: pt = [pt1 (o, j) pt2] and yield(pt) = yield(pt1) o yield(pt2). *)
   - simpl.
+    apply wf_pos_tree_size in H as ?.
+    apply wf_pos_tree_size in H1 as ?.
     inv H0.
-    + apply wf_pos_tree_size in H.
-      apply list_lookup_middle.
+    (* CASE: s = o and i = j *)
+    + apply list_lookup_middle.
       lia.
+    (* CASE: s is in pt1 *)
     + apply lookup_app_l_Some.
       auto.
-    + eapply symbol_between_indices in H4 as ?; [|eassumption].
-      destruct H0.
+    (* CASE: s is in pt2 *)
+    + eapply symbol_between_indices in H6 as ?; [|eassumption].
       apply wf_pos_tree_size in H.
       apply wf_pos_tree_size in H1.
-      apply IHwf_pos_tree2 in H4.
-      rewrite <- H4.
+      apply IHwf_pos_tree2 in H6.
+      rewrite <- H6.
       rewrite cons_middle.
       rewrite app_assoc.
-      replace (i - S j) with (i - i0 - length (yield (unpos pt1) ++ [inr o])).
+      replace (i - S (i0 + length (yield (unpos pt1))))
+        with (i - i0 - length (yield (unpos pt1) ++ [inr o])).
       apply lookup_app_r.
       rewrite app_length.
       simpl.
@@ -74,43 +86,43 @@ Proof.
       lia.
 Qed.
 
+(* If a symbol s is in the i-th position of the yield of a well-formed pos_tree pt between
+   n0 and n, then s is the (n0 + i)th position of the tree. *)
 Lemma yield_pos pt n0 n s i :
   wf_pos_tree n0 pt n ->
-  (yield (unpos pt)) !! i = Some s -> nth_symbol (n0 + i) s pt.
+  (yield (unpos pt)) !! i = Some s -> ith_symbol (n0 + i) s pt.
 Proof.
   intro. revert i.
   induction H; intros; simpl in *; simplify_list_eq.
+  (* CASE: pt = (l, n0) *)
   - replace (i + 0) with i; [|lia].
-    apply L_nth.
-
+    apply L_ith.
+  (* CASE: pt = [pt1 (o, j) pt2] *)
   - apply wf_pos_tree_size in H as ?.
     apply wf_pos_tree_size in H0 as ?.
-
     apply lookup_app_Some in H1.
     destruct H1.
-    + apply Symbol_nth1.
-      apply IHwf_pos_tree1.
-      assumption.
+    (* CASE: s is in yield(pt1) *)
+    + auto with pos_tree.
     + destruct H1.
-      destruct (i0 - length (yield (unpos pt1))) eqn:E.
-      * simplify_list_eq.
-        replace i0 with (length (yield (unpos pt1))); [|lia].
-        apply O_nth.
-      * simplify_list_eq.
-        apply Symbol_nth2.
+      destruct (i0 - length (yield (unpos pt1))) eqn:E; simplify_list_eq.
+    (* CASE: s = o *)
+      * replace i0 with (length (yield (unpos pt1))); [|lia].
+        apply O_ith.
+    (* CASE: s is in yield(pt2) *)
+      * apply S_ith_r.
         apply IHwf_pos_tree2 in H4.
-        replace (i + i0) with (S (i + length (yield (unpos pt1)) + n)).
-        assumption.
-        lia.
+        replace (i + i0) with (S (i + length (yield (unpos pt1)) + n)); [auto|lia].
 Qed.
 
+(* Two pos_trees are position equivalent if and only if they have equal yields. *)
 Lemma pos_equivalence_yields pt1 pt2 n0 n :
   wf_pos_tree n0 pt1 n -> wf_pos_tree n0 pt2 n ->
   (pos_equivalent pt1 pt2 <-> yield (unpos pt1) = yield (unpos pt2)).
 Proof.
+  (* Simple proof by Lemmas pos_yield and yield_pos. *)
   intros.
   split.
-
   - intros.
     unfold pos_equivalent in H1.
     apply nth_error_equality.
@@ -128,7 +140,6 @@ Proof.
       eapply pos_yield in H2; [|eassumption].
       replace (n0 + i - n0) with i in H2; [|lia].
       assumption.
-
   - unfold pos_equivalent.
     intros.
     split; intros.
@@ -148,6 +159,7 @@ Proof.
       assumption.
 Qed.
 
+(* The pos function actually gives back a well-formed pos_tree. *)
 Lemma pos_wf_pos_tree t pt n0 n :
   pos t n0 = (pt, n) -> wf_pos_tree n0 pt n.
 Proof.
@@ -161,6 +173,7 @@ Proof.
     apply Wfpos_PINode; auto.
 Qed.
 
+(* Unpos is the injective function of pos. *)
 Lemma pos_unpos t n0 p n :
   pos t n0 = (p, n) -> unpos p = t.
 Proof.
@@ -178,26 +191,13 @@ Proof.
     reflexivity.
 Qed.
 
-Lemma pos_tree_parse_tree (P : @parse_tree L O -> Prop) :
-  (forall n0 pt n, wf_pos_tree n0 pt n -> P (unpos pt)) -> forall t, P t.
-Proof.
-  intros.
-  remember (pos t 0) as x.
-  destruct x.
-  specialize H with (n0 := 0) (pt := p) (n := n).
-  symmetry in Heqx.
-  apply pos_wf_pos_tree in Heqx as ?.
-  apply H in H0.
-  apply pos_unpos in Heqx.
-  rewrite Heqx in H0.
-  assumption.
-Qed.
-
-Lemma symbol_nth_subtree_l n0 n i j s o pt1 pt2 :
-  wf_pos_tree n0 (PINode pt1 o i pt2) n ->
-  nth_symbol j s (PINode pt1 o i pt2) ->
-  j < i ->
-  nth_symbol j s pt1.
+(* Suppose we have a pos_tree [pt1 (o, j) pt2]. If a symbol is in the i-th position of
+   the tree and i < j, then the symbol must be in pt1. *)
+Lemma symbol_ith_subtree_l n0 n i j s o pt1 pt2 :
+  wf_pos_tree n0 (PINode pt1 o j pt2) n ->
+  ith_symbol i s (PINode pt1 o j pt2) ->
+  i < j ->
+  ith_symbol i s pt1.
 Proof.
   intros.
   inv H.
@@ -209,11 +209,13 @@ Proof.
     lia.
 Qed.
 
-Lemma symbol_nth_subtree_r n0 n i j s o pt1 pt2 :
-  wf_pos_tree n0 (PINode pt1 o i pt2) n ->
-  nth_symbol j s (PINode pt1 o i pt2) ->
-  j > i ->
-  nth_symbol j s pt2.
+(* Suppose we have a pos_tree [pt1 (o, j) pt2]. If a symbol is in the i-th position of
+   the tree and i > j, then the symbol must be in pt2. *)
+Lemma symbol_ith_subtree_r n0 n i j s o pt1 pt2 :
+  wf_pos_tree n0 (PINode pt1 o j pt2) n ->
+  ith_symbol i s (PINode pt1 o j pt2) ->
+  i > j ->
+  ith_symbol i s pt2.
 Proof.
   intros.
   inv H.
@@ -225,6 +227,7 @@ Proof.
   - assumption.
 Qed.
 
+(* For two pos_trees where the top operator and index is (o, i). *)
 Lemma pos_equivalent_subtrees pt1 pt1_1 pt1_2 pt2 pt2_1 pt2_2 o i n0 n :
   pt1 = PINode pt1_1 o i pt1_2 ->
   pt2 = PINode pt2_1 o i pt2_2 ->
@@ -233,6 +236,7 @@ Lemma pos_equivalent_subtrees pt1 pt1_1 pt1_2 pt2 pt2_1 pt2_2 o i n0 n :
   pos_equivalent pt1 pt2 ->
   pos_equivalent pt1_1 pt2_1 /\ pos_equivalent pt1_2 pt2_2.
 Proof.
+  (* By the two above Lemmas. *)
   intros. subst.
   unfold pos_equivalent in *.
   split; intros.
@@ -243,22 +247,20 @@ Proof.
       inv H1'.
       eapply symbol_between_indices in H3 as ?; [|eassumption].
       destruct H4.
-      assert (nth_symbol i0 s (PINode pt1_1 o i pt1_2)). {
-        apply Symbol_nth1.
-        assumption.
+      assert (ith_symbol i0 s (PINode pt1_1 o i pt1_2)). {
+        auto with pos_tree.
       }
       apply H in H6.
-      eauto using symbol_nth_subtree_l.
+      eauto using symbol_ith_subtree_l.
     + assert (H2' := H2).
       inv H2'.
       eapply symbol_between_indices in H3 as ?; [|eassumption].
       destruct H4.
-      assert (nth_symbol i0 s (PINode pt2_1 o i pt2_2)). {
-        apply Symbol_nth1.
-        assumption.
+      assert (ith_symbol i0 s (PINode pt2_1 o i pt2_2)). {
+        auto with pos_tree.
       }
       apply H0 in H6.
-      eauto using symbol_nth_subtree_l.
+      eauto using symbol_ith_subtree_l.
   - specialize H3 with (s := s) (i0 := i0).
     destruct H3.
     split; intros.
@@ -266,24 +268,23 @@ Proof.
       inv H1'.
       eapply symbol_between_indices in H3 as ?; [|eassumption].
       destruct H4.
-      assert (nth_symbol i0 s (PINode pt1_1 o i pt1_2)). {
-        apply Symbol_nth2.
-        assumption.
+      assert (ith_symbol i0 s (PINode pt1_1 o i pt1_2)). {
+        auto with pos_tree.
       }
       apply H in H6.
-      eauto using symbol_nth_subtree_r.
+      eauto using symbol_ith_subtree_r.
     + assert (H2' := H2).
       inv H2'.
       eapply symbol_between_indices in H3 as ?; [|eassumption].
       destruct H4.
-      assert (nth_symbol i0 s (PINode pt2_1 o i pt2_2)). {
-        apply Symbol_nth2.
-        assumption.
+      assert (ith_symbol i0 s (PINode pt2_1 o i pt2_2)). {
+        auto with pos_tree.
       }
       apply H0 in H6.
-      eauto using symbol_nth_subtree_r.
+      eauto using symbol_ith_subtree_r.
 Qed.
 
+(* Position eequivalence is a transitive relation. *)
 Lemma pos_equivalent_transitive pt1 pt2 pt3 :
   pos_equivalent pt1 pt2 -> pos_equivalent pt2 pt3 -> pos_equivalent pt1 pt3.
 Proof.
