ReorderingTheorems.v
@@ -9,17 +9,33 @@ Implicit Types s : L + O.
 Implicit Types t : @parse_tree L O.
 Implicit Types pt : @pos_tree L O.
 
+Ltac super_simpl := try simpl in *; try simplify_list_eq; try reflexivity.
+
+Lemma reorder_step_preserves_yields t t' :
+  reorder_step t t' -> yield t = yield t'.
+Proof.
+  intros. induction H; super_simpl.
+  - rewrite IHreorder_step. reflexivity.
+  - rewrite IHreorder_step. reflexivity.
+Qed.
+
+Lemma reorder_preserves_yield t t' :
+  reorder t t' -> yield t = yield t'.
+Proof.
+  unfold reorder. intros.
+  induction H.
+  - reflexivity.
+  - rewrite <- IHrtc.
+    apply reorder_step_preserves_yields.
+    assumption.
+Qed.
+
+(* Reordering is a symmetric relation. *)
 Lemma reorder_step_pos_symmetry pt1 pt2 :
   reorder_step_pos pt1 pt2 -> reorder_step_pos pt2 pt1.
 Proof.
   intros.
-  induction H.
-  - apply PRI_RL.
-  - apply PRI_LR.
-  - apply PRI_pt1.
-    assumption.
-  - apply PRI_pt2.
-    assumption.
+  induction H; auto with reordering.
 Qed.
 
 Lemma reorder_pos_symmetry pt1 pt2 :
@@ -36,6 +52,7 @@ Proof.
       * apply rtc_refl.
 Qed.
 
+(* Reordering preserves well-formedness of trees *)
 Lemma reorder_step_pos_wf_pos_tree n0 pt n pt' :
   wf_pos_tree n0 pt n -> reorder_step_pos pt pt' -> wf_pos_tree n0 pt' n.
 Proof.
@@ -97,13 +114,10 @@ Proof.
   - unfold pos_equivalent.
     auto.
   - apply reorder_step_pos_preserves_position in H.
-    unfold pos_equivalent in *.
-    intros.
-    split; intros.
-    + apply IHrtc. apply H. assumption.
-    + apply H. apply IHrtc. assumption.
+    eapply pos_equivalent_transitive; eauto.
 Qed.
 
+(* We can always reorder the left subtree. *)
 Lemma reorder_pos_subtree_l pt1 o i pt2 pt1' :
   reorder_pos pt1 pt1' ->
   reorder_pos (PINode pt1 o i pt2) (PINode pt1' o i pt2).
@@ -111,12 +125,10 @@ Proof.
   intros.
   induction H.
   - apply rtc_refl.
-  - eapply rtc_l.
-    + apply PRI_pt1.
-      eassumption.
-    + assumption.
+  - eapply rtc_l; eauto with reordering.
 Qed.
 
+(* We can always reorder the right subtree. *)
 Lemma reorder_pos_subtree_r pt1 o i pt2 pt2' :
   reorder_pos pt2 pt2' ->
   reorder_pos (PINode pt1 o i pt2) (PINode pt1 o i pt2').
@@ -124,19 +136,19 @@ Proof.
   intros.
   induction H.
   - apply rtc_refl.
-  - eapply rtc_l.
-    + apply PRI_pt2.
-      eassumption.
-    + assumption.
+  - eapply rtc_l; eauto with reordering.
 Qed.
 
-Lemma reorder_pos_nth_op_top i o pt :
-  nth_symbol i (inr o) pt ->
+(* We can always reorder a pos_tree such that any operator ends up on top. *)
+Lemma reorder_pos_ith_op_top i o pt :
+  ith_symbol i (inr o) pt ->
   exists pt1 pt2, reorder_pos pt (PINode pt1 o i pt2).
 Proof.
   intros.
   induction pt; inv H.
+  (* CASE: (o, i) is already one top. *)
   - eexists. eexists. eapply rtc_refl.
+  (* CASE: (o, i) is in the left subtree. *)
   - apply IHpt1 in H2.
     destruct H2. destruct H.
     eexists. eexists.
@@ -145,6 +157,7 @@ Proof.
       eassumption.
     + eapply rtc_once.
       eapply PRI_LR.
+  (* CASE: (o, i) is in the right subtree. *)
   - apply IHpt2 in H2.
     destruct H2. destruct H.
     eexists. eexists.
@@ -155,6 +168,7 @@ Proof.
       eapply PRI_RL.
 Qed.
 
+(* We can always reorder two position equivalent trees with each other. *)
 Lemma pos_equivalent_reorder_pos pt1 pt2 n0 n :
   wf_pos_tree n0 pt1 n -> wf_pos_tree n0 pt2 n ->    
   pos_equivalent pt1 pt2 ->
@@ -163,42 +177,50 @@ Proof.
   intro. revert pt2.
   induction H.
 
+  (* CASE: pt1 = (l, i) *)
   - intros.
     unfold pos_equivalent in H0.
     destruct pt2.
+    (* CASE: pt2 = (l2, i2) *)
     + specialize H0 with (s := inl l) (i0 := i).
       destruct H0.
-      assert (@nth_symbol L O i (inl l) (PANode l i)). apply L_nth.
+      assert (@ith_symbol L O i (inl l) (PANode l i)). { apply L_ith. }
       apply H0 in H2.
       inv H2.
       apply rtc_refl.
+    (* CASE: pt2 = [pt21 (o, j) pt22]. Impossible case by position equivalence. *)
     + specialize H0 with (s := inr o) (i0 := n).
       destruct H0.
-      assert (nth_symbol n (inr o) (PINode pt2_1 o n pt2_2)). apply O_nth.
+      assert (ith_symbol n (inr o) (PINode pt2_1 o n pt2_2)). { apply O_ith. }
       apply H1 in H2.
       inv H2.
 
+  (* CASE: pt1 = [pt11 (o, i) pt12] *)
   - intros.
 
+    (* This means (o, i) is also in pt2. *)
     assert (H2' := H2).
     unfold pos_equivalent in H2'.
     specialize H2' with (s := inr o) (i := j).
-    assert (nth_symbol j (inr o) (PINode pt1 o j pt2)). apply O_nth.
+    assert (ith_symbol j (inr o) (PINode pt1 o j pt2)). { apply O_ith. }
     apply H2' in H3. clear H2'.
-
-    apply reorder_pos_nth_op_top in H3.
-    destruct H3.
-    destruct H3.
+    (* This means we can reorder the operator to the top of pt2. *)
+    apply reorder_pos_ith_op_top in H3.
+    destruct H3. destruct H3.
+    (* This new tree is also position equivalent. *)
     eapply reorder_pos_wf_pos_tree in H3 as ?; eauto.
     inv H4.
     eapply reorder_pos_preserves_position in H3 as ?; eauto.
     assert (pos_equivalent (PINode pt1 o j pt2) (PINode x o j x0)). {
       eapply pos_equivalent_transitive; eassumption.
     }
+    (* The subtrees are position equivalent with each other. *)
     eapply pos_equivalent_subtrees in H5; eauto with pos_tree.
     destruct H5.
+    (* By induction hypothesis we can reorder the subtrees to each other. *)
     apply IHwf_pos_tree1 in H5; auto.
     apply IHwf_pos_tree2 in H6; auto.
+    (* In conclusion, we can reorder everything to each other. *)
     eapply rtc_transitive.
     eapply reorder_pos_subtree_l.
     eassumption.
@@ -209,15 +231,12 @@ Proof.
     assumption.
 Qed.
 
+(* Reordering with pos_trees is the same as reordering with ordinary parse_trees *)
 Lemma reorder_step_pos_unpos_reorder_step pt pt' :
   reorder_step_pos pt pt' -> reorder_step (unpos pt) (unpos pt').
 Proof.
   intros.
-  induction H; simpl.
-  - apply RI_LR.
-  - apply RI_RL.
-  - apply RI_t1. assumption.
-  - apply RI_t2. assumption.
+  induction H; simpl; auto with reordering.
 Qed.
 
 Lemma reorder_pos_unpos_reorder pt pt' :
@@ -226,20 +245,22 @@ Proof.
   intros.
   induction H.
   - apply rtc_refl.
-  - eapply rtc_l.
-    + apply reorder_step_pos_unpos_reorder_step.
-      eassumption.
-    + assumption.
+  - eapply rtc_l; eauto using reorder_step_pos_unpos_reorder_step.
 Qed.
 
+(* Proving that position equivalence implies reordering, is the same as proving that
+   yield equivalence (for parse_trees) implies reordering. *)
 Lemma reorder_pos_forall_unpos :
   (forall pt pt' n0 n,
     wf_pos_tree n0 pt n -> wf_pos_tree n0 pt' n ->
     pos_equivalent pt pt' -> reorder_pos pt pt') ->
   (forall t t', yield t = yield t' -> reorder t t').
 Proof.
+  (* By the following facts:
+     - Yield equivalence is position equivalence.
+     - All parse_trees can be transformed into pos_trees with the pos function.
+     - unpos is the injective function of pos. *)
   intros.
-
   remember (pos t 0) as x.
   destruct x.
   symmetry in Heqx.
